src/ListIds.v
@@ -36,6 +36,8 @@ Proof.
     assumption.
 Qed.
 
+Hint Resolve in_list_id_or_append.
+
 Lemma in_list_id_or_append_inversion : forall x l1 l2,
     in_list_id x (l1 ++ l2) = true ->
     in_list_id x l1 = true \/ in_list_id x l2 = true.
@@ -51,13 +53,28 @@ Proof.
     auto.
 Qed.
 
-Lemma in_list_id_cons : forall x l a,
-    in_list_id x l = true ->
-    in_list_id x (a::l) = true.
+Hint Resolve in_list_id_or_append_inversion.
+
+Lemma in_list_id_cons_true : forall x l a,
+    in_list_id x l = true -> in_list_id x (a::l) = true.
 Proof.
   intros.
   mysimp.
 Qed.
+
+Hint Resolve in_list_id_cons_true.
+
+Lemma in_list_id_cons_false : forall x l a,
+    in_list_id x (a::l) = false -> in_list_id x l = false.
+  Proof.
+  intros.
+  simpl in H.
+  destruct (eq_id_dec a x);
+  mysimp.
+  inversion H.
+Qed.
+
+Hint Resolve in_list_id_cons_false.
 
 Lemma in_list_id_append_comm_true :
   forall x l1 l2, in_list_id x (l1 ++ l2) = true ->
@@ -69,6 +86,8 @@ Proof.
   destruct H; mysimp.
 Qed.
 
+Hint Resolve in_list_id_append_comm_true.
+
 Lemma in_list_id_append1 :
   forall x l1 l2, in_list_id x l1 = true ->
              in_list_id x (l1 ++ l2) = true.
@@ -79,6 +98,8 @@ Proof.
   auto.
 Qed.
 
+Hint Resolve in_list_id_append1.
+
 Lemma in_list_id_append2 :
   forall x l1 l2, in_list_id x l2 = true ->
              in_list_id x (l1 ++ l2) = true.
@@ -88,6 +109,8 @@ Proof.
   right.
   auto.
 Qed.
+
+Hint Resolve in_list_id_append2.
 
 Lemma in_list_id_and_append : forall x l1 l2,
     in_list_id x l1 = false /\ in_list_id x l2 = false ->
@@ -102,6 +125,8 @@ Proof.
     assumption.
 Qed.
 
+Hint Resolve in_list_id_and_append.
+
 Lemma in_list_id_and_append_inversion : forall x l1 l2,
     in_list_id x (l1 ++ l2) = false ->
     in_list_id x l1 = false /\ in_list_id x l2 = false.
@@ -111,6 +136,8 @@ Proof.
   try (simpl in H; destruct (eq_id_dec x x); intuition);
   try (destruct (eq_id_dec a x); intuition).
 Qed.
+
+Hint Resolve in_list_id_and_append_inversion.
 
 Lemma in_list_id_append_comm_false :
   forall x l1 l2, in_list_id x (l1 ++ l2) = false ->
@@ -122,6 +149,8 @@ Proof.
   destruct H; mysimp.
 Qed.
 
+Hint Resolve in_list_id_append_comm_false.
+
 Lemma in_list_id_append_inversion1 :
   forall x l1 l2, (in_list_id x (l1 ++ l2) = false ->
               in_list_id x l1 = false).
@@ -131,6 +160,8 @@ Proof.
   - reflexivity.
   - simpl in *. destruct (eq_id_dec a x); intuition.
 Qed.
+
+Hint Resolve in_list_id_append_inversion1.
 
 Lemma in_list_id_append_inversion2 :
   forall x l1 l2, (in_list_id x (l1 ++ l2) = false ->
@@ -143,6 +174,8 @@ Proof.
     destruct (eq_id_dec a x); intuition.
 Qed.
 
+Hint Resolve in_list_id_append_inversion2.
+
 (** index of a id is in a list *)
 
 Fixpoint index_list_id_aux (count i : id) (l : list id) : option id :=
@@ -150,6 +183,8 @@ Fixpoint index_list_id_aux (count i : id) (l : list id) : option id :=
   | nil => None
   | x::l' => if eq_id_dec x i then Some count else index_list_id_aux (S count) i l'
   end.
+
+Hint Resolve index_list_id_aux.
 
 Definition index_list_id (i:id) (l:list id) := index_list_id_aux 0 i l.
   
@@ -215,6 +250,8 @@ Proof.
   omega.
 Qed.
 
+Hint Resolve max_list_ids'_eq.
+
 Lemma max_list_ids'_false : forall  x l x0 P,  max_list_ids' l x = exist _ x0 P -> x0 < x -> False.
 Proof.
   intros.
@@ -230,6 +267,8 @@ Proof.
     omega.
 Qed.
 
+Hint Resolve max_list_ids'_false.
+
 Lemma in_list_id_le_ex : forall l p i, (forall x : id, in_list_id x (p :: l) = true -> x < i) -> p < i.
 Proof.
   intros.
@@ -237,6 +276,8 @@ Proof.
   simpl in H.
   destruct (eq_id_dec p p); intuition.
 Qed.
+
+Hint Resolve in_list_id_le_ex.
 
 Definition max_ids (i1 i2 : id) : id := if le_gt_dec i1 i2 then i2 else i1.
 
@@ -264,11 +305,14 @@ Proof.
     mysimp.
 Qed.
 
+Hint Resolve apply_subst_dom_false.
+
 Lemma not_in_img: forall (s: substitution) (st x: id),
     st <> x -> 
     in_list_id st (img_ids s) = false ->
     in_list_id st (ids_ty (apply_subst s (var x))) = false.
 Proof.
+  intros.
   induction s. 
   - simpl in |- *. intros. mysimp.
   - destruct a.
@@ -276,15 +320,17 @@ Proof.
     destruct (eq_id_dec i x).
     + unfold img_ids in H0. simpl in H0.
       apply in_list_id_and_append_inversion in H0; destruct H0; auto.
-      induction t.
-      apply IHs. simpl in H0. destruct (eq_id_dec i0 st); intuition; auto.
-      unfold img_ids. auto.
-      rewrite apply_subst_con. reflexivity.
-      rewrite apply_subst_arrow.
-      simpl.
-      eapply in_list_id_and_append.
-      simpl in H0.
-      apply in_list_id_and_append_inversion in H0; destruct H0; auto.
-    + unfold img_ids in H0. simpl in H0.
-      apply in_list_id_and_append_inversion in H0; destruct H0; auto.
+    + simpl in *. eapply IHs; eauto. 
+      induction t; simpl in *; mysimp; eauto.
+      cases (find_subst s x); simpl in *; eauto. 
+      unfold img_ids in H0. simpl in H0.
+      eauto.
+      destruct (eq_id_dec x st);
+      eauto.
+      unfold img_ids in H0. simpl in H0.
+      eauto.
+      unfold img_ids in H0. simpl in H0.
+      eauto.
 Qed.
+
+Hint Resolve not_in_img.
